Wavelet/Semantics.lean
@@ -3,5 +3,6 @@ import Wavelet.Semantics.Lts
 import Wavelet.Semantics.Link
 import Wavelet.Semantics.OpInterp
 import Wavelet.Semantics.PCM
+import Wavelet.Semantics.Confluence
 
 /-! Common definitions for semantics. -/
