Wavelet/Semantics/Confluence.lean
@@ -1,0 +1,31 @@
+import Wavelet.Semantics.Defs
+
+/-! Some definitions for confluence. -/
+
+namespace Wavelet.Semantics
+
+/-- Strong confluence of `c` when the labels are restricted
+by the compatibility relation `Compat`. -/
+def Lts.StronglyConfluentAt
+  {C : Type u} {E : Type v}
+  (lts : Lts C E)
+  (c : C)
+  (Compat : E → E → Prop) : Prop :=
+  ∀ {c₁ c₂ : C} {l₁ l₂ : E},
+    lts.Step c l₁ c₁ →
+    lts.Step c l₂ c₂ →
+    Compat l₁ l₂ →
+    c₁ = c₂ ∨
+    ∃ c',
+      lts.Step c₁ l₂ c' ∧
+      lts.Step c₂ l₁ c'
+
+/-- Strong confluence of an LTS when restricted to a subset of states. -/
+def Lts.StronglyConfluent
+  {C : Type u} {E : Type v}
+  (lts : Lts C E)
+  (States : C → Prop)
+  (Compat : E → E → Prop) : Prop :=
+  ∀ {c : C}, States c → lts.StronglyConfluentAt c Compat
+
+end Wavelet.Semantics
